compiler/backend/passes/proofs/thunk_case_liftProofScript.sml
@@ -38,81 +38,81 @@ Inductive exp_rel:
      exp_rel z1 z2 ⇒
        exp_rel (Tick (If (IsEq s i T x1) y1 z1))
                (Let (SOME w) (Tick (Tick x2))
-                             (If (IsEq s i T x2) y2 z2))) ∧
+                             (If (IsEq s i T x2) y2 z2)))
 (* Boilerplate: *)
 [exp_rel_App:]
   (∀f g x y.
      exp_rel f g ∧
      exp_rel x y ⇒
-       exp_rel (App f x) (App g y)) ∧
+       exp_rel (App f x) (App g y))
 [exp_rel_Lam:]
   (∀s x y.
      exp_rel x y ⇒
-       exp_rel (Lam s x) (Lam s y)) ∧
+       exp_rel (Lam s x) (Lam s y))
 [exp_rel_Letrec:]
   (∀f g x y.
      LIST_REL (λ(fn,x) (gn,y). fn = gn ∧ exp_rel x y) f g ∧
      exp_rel x y ⇒
-       exp_rel (Letrec f x) (Letrec g y)) ∧
+       exp_rel (Letrec f x) (Letrec g y))
 [exp_rel_Let:]
   (∀bv x1 y1 x2 y2.
      exp_rel x1 x2 ∧
      exp_rel y1 y2 ⇒
-       exp_rel (Let bv x1 y1) (Let bv x2 y2)) ∧
+       exp_rel (Let bv x1 y1) (Let bv x2 y2))
 [exp_rel_If:]
   (∀x1 x2 y1 y2 z1 z2.
      LIST_REL exp_rel [x1;y1;z1] [x2;y2;z2] ⇒
-       exp_rel (If x1 y1 z1) (If x2 y2 z2)) ∧
+       exp_rel (If x1 y1 z1) (If x2 y2 z2))
 [exp_rel_Prim:]
   (∀op xs ys.
      LIST_REL exp_rel xs ys ⇒
-       exp_rel (Prim op xs) (Prim op ys)) ∧
+       exp_rel (Prim op xs) (Prim op ys))
 [exp_rel_Monad:]
   (∀mop xs ys.
      LIST_REL exp_rel xs ys ⇒
-       exp_rel (Monad mop xs) (Monad mop ys)) ∧
+       exp_rel (Monad mop xs) (Monad mop ys))
 [exp_rel_Delay:]
   (∀x y.
      exp_rel x y ⇒
-       exp_rel (Delay x) (Delay y)) ∧
+       exp_rel (Delay x) (Delay y))
 [exp_rel_Force:]
   (∀x y.
      exp_rel x y ⇒
-       exp_rel (Force x) (Force y)) ∧
+       exp_rel (Force x) (Force y))
 [exp_rel_MkTick:]
   (∀x y.
      exp_rel x y ⇒
-       exp_rel (MkTick x) (MkTick y)) ∧
+       exp_rel (MkTick x) (MkTick y))
 [exp_rel_Var:]
   (∀v.
-     exp_rel (Var v) (Var v)) ∧
+     exp_rel (Var v) (Var v))
 [exp_rel_Value:]
   (∀v w.
      v_rel v w ⇒
-     exp_rel (Value v) (Value w)) ∧
+     exp_rel (Value v) (Value w))
 [v_rel_Atom:]
   (∀x.
-     v_rel (Atom x) (Atom x)) ∧
+     v_rel (Atom x) (Atom x))
 [v_rel_Constructor:]
   (∀vs ws.
      LIST_REL v_rel vs ws ⇒
-       v_rel (Constructor s vs) (Constructor s ws)) ∧
+       v_rel (Constructor s vs) (Constructor s ws))
 [v_rel_Monadic:]
   (∀mop xs ys.
      LIST_REL exp_rel xs ys ⇒
-       v_rel (Monadic mop xs) (Monadic mop ys)) ∧
+       v_rel (Monadic mop xs) (Monadic mop ys))
 [v_rel_Closure:]
   (∀s x y.
      exp_rel x y ⇒
-       v_rel (Closure s x) (Closure s y)) ∧
+       v_rel (Closure s x) (Closure s y))
 [v_rel_DoTick:]
   (∀v w.
      v_rel v w ⇒
-       v_rel (DoTick v) (DoTick w)) ∧
+       v_rel (DoTick v) (DoTick w))
 [v_rel_Recclosure:]
   (∀f g n.
      LIST_REL (λ(fn,x) (gn,y). fn = gn ∧ exp_rel x y) f g ⇒
-       v_rel (Recclosure f n) (Recclosure g n)) ∧
+       v_rel (Recclosure f n) (Recclosure g n))
 [v_rel_Thunk:]
   (∀x y.
      exp_rel x y ⇒
@@ -643,47 +643,47 @@ Inductive compile_rel:
      compile_rel y1 y2 ∧
      compile_rel z1 z2 ⇒
        compile_rel (If (IsEq s i T x1) y1 z1)
-                   (Let (SOME w) x2 (If (IsEq s i T x2) y2 z2))) ∧
+                   (Let (SOME w) x2 (If (IsEq s i T x2) y2 z2)))
 (* Boilerplate: *)
 [~App:]
   (∀f g x y.
      compile_rel f g ∧
      compile_rel x y ⇒
-       compile_rel (App f x) (App g y)) ∧
+       compile_rel (App f x) (App g y))
 [~Lam:]
   (∀s x y.
      compile_rel x y ⇒
-       compile_rel (Lam s x) (Lam s y)) ∧
+       compile_rel (Lam s x) (Lam s y))
 [~Letrec:]
   (∀f g x y.
      LIST_REL (λ(fn,x) (gn,y). fn = gn ∧ ok_bind x ∧ compile_rel x y) f g ∧
      compile_rel x y ⇒
-       compile_rel (Letrec f x) (Letrec g y)) ∧
+       compile_rel (Letrec f x) (Letrec g y))
 [~Let:]
   (∀bv x1 y1 x2 y2.
      compile_rel x1 x2 ∧
      compile_rel y1 y2 ⇒
-       compile_rel (Let bv x1 y1) (Let bv x2 y2)) ∧
+       compile_rel (Let bv x1 y1) (Let bv x2 y2))
 [~If:]
   (∀x1 x2 y1 y2 z1 z2.
      LIST_REL compile_rel [x1;y1;z1] [x2;y2;z2] ⇒
-       compile_rel (If x1 y1 z1) (If x2 y2 z2)) ∧
+       compile_rel (If x1 y1 z1) (If x2 y2 z2))
 [~Prim:]
   (∀op xs ys.
      LIST_REL compile_rel xs ys ⇒
-       compile_rel (Prim op xs) (Prim op ys)) ∧
+       compile_rel (Prim op xs) (Prim op ys))
 [~Monad:]
   (∀mop xs ys.
      LIST_REL compile_rel xs ys ⇒
-       compile_rel (Monad mop xs) (Monad mop ys)) ∧
+       compile_rel (Monad mop xs) (Monad mop ys))
 [~Delay:]
   (∀x y.
      compile_rel x y ⇒
-       compile_rel (Delay x) (Delay y)) ∧
+       compile_rel (Delay x) (Delay y))
 [~Force:]
   (∀x y.
      compile_rel x y ⇒
-       compile_rel (Force x) (Force y)) ∧
+       compile_rel (Force x) (Force y))
 [~Var:]
   (∀v.
      compile_rel (Var v) (Var v))
